generalize remdups from nat to 'a

Examples/Remdups.thy
@@ -13,7 +13,7 @@ definition body_time :: "nat \<Rightarrow> nat" where
 
 definition "rd_ta as = (\<lambda>(xs,ys,S). length xs * body_time (length as))"
 
-definition rd_impl1 :: "nat list \<Rightarrow> (nat list) nrest" where
+definition rd_impl1 :: "('a::{heap,linorder}) list \<Rightarrow> ('a list) nrest" where
 "rd_impl1 as = do {
   ys \<leftarrow> mop_empty_list 12;
   S \<leftarrow> mop_set_empty 1;
@@ -96,7 +96,7 @@ lemma hn_refine_tl[sepref_fr_rules]: " hn_refine (hn_val Id s' s)
 (* synthesize *) 
 
 context 
-  fixes as::"nat list"
+  fixes as::"('a::{heap,linorder}) list"
   notes [[sepref_register_adhoc as]]
   notes [sepref_import_param] = IdI[of as] 
 begin
@@ -104,8 +104,8 @@ begin
 declare rbt_search_time_logN_mono [intro]
 declare rbt_insert_logN_mono [intro]
 
-sepref_definition remdups_impl is "uncurry0 (rd_impl1 as)" :: "unit_assn\<^sup>k \<rightarrow>\<^sub>a da_assn nat_assn"
-  unfolding rd_impl1_def whileIET_def
+sepref_definition remdups_impl is "uncurry0 (rd_impl1 as)" :: "unit_assn\<^sup>k \<rightarrow>\<^sub>a da_assn id_assn"
+  unfolding rd_impl1_def whileIET_def 
   apply sepref_dbg_keep 
   done
 print_theorems
@@ -116,9 +116,9 @@ thm  hnr_refine[OF rd_impl1_correct  remdups_impl.refine[to_hnr],to_hfref]
 thm extract_cost_ub[OF hnr_refine[OF rd_impl1_correct  remdups_impl.refine[to_hnr]], where Cost_ub="remdups_time (length as)", simplified in_ran_emb_special_case,   simplified ]
 
 
-lemma "<$ (remdups_time (length as))> 
+lemma remdups_rule: "<$ (remdups_time (length as))> 
           remdups_impl 
-        <\<lambda>r. \<exists>\<^sub>Ara. da_assn nat_assn ra r * \<up> (set as = set ra \<and> distinct ra)>\<^sub>t"
+        <\<lambda>r. \<exists>\<^sub>Ara. da_assn id_assn ra r * \<up> (set as = set ra \<and> distinct ra)>\<^sub>t"
   using  extract_cost_ub[OF hnr_refine[OF rd_impl1_correct  remdups_impl.refine[to_hnr]], where Cost_ub="remdups_time (length as)", simplified in_ran_emb_special_case,   simplified ]
   by auto
 (*
